code/experimental/rsapss/Hacl.Impl.Bignum.Misc.fst
@@ -4,10 +4,13 @@ open FStar.HyperStack
 open FStar.HyperStack.ST
 open FStar.Mul
 
+open Lib.ByteBuffer
 open Lib.IntTypes
 open Lib.Buffer
+open Lib.PrintBuffer
 
 open Hacl.Impl.Bignum.Core
+open Hacl.Impl.Bignum.Convert
 open Hacl.Spec.Bignum
 
 val bn_assign_uint64:
@@ -22,3 +25,34 @@ let bn_assign_uint64 #len a x =
   if len >. 1ul then memset (sub a 1ul (len -! 1ul)) (uint 0) (len -! 1ul);
   let h = FStar.HyperStack.ST.get () in
   assume (as_snat h a = v x)
+
+
+//////// Some debugging, at least for the time being
+
+noextract inline_for_extraction
+let debugOn = false
+
+// Prints in big endian, both with respect to uint64 chunks, and within them.
+val print_lbignum:
+     #aLen:bn_len
+  -> a:lbignum aLen
+  -> ST unit (requires fun h -> live h a) (ensures fun h0 _ h1 -> h0 == h1)
+let print_lbignum #aLen a =
+  assume (8 * v aLen < max_size_t);
+  push_frame ();
+  let bytes_n = aLen *! 8ul in
+  let bytes = create bytes_n (uint 0) in
+  let a' = bignum_to_bytes a bytes in
+  print_bytes bytes_n bytes;
+  pop_frame ();
+  admit()
+
+noextract inline_for_extraction
+val trace_lbignum:
+     #aLen:bn_len
+  -> a:lbignum aLen
+  -> ST unit (requires fun h -> live h a) (ensures fun h0 _ h1 -> h0 == h1)
+let trace_lbignum #aLen a = if debugOn then print_lbignum a else ()
+
+noextract inline_for_extraction
+let trace (s:string) = if debugOn then C.String.print (C.String.of_literal s) else ()
